---
layout: default
title : Rules for Addition
---

## Rules for Addition

### 개념 요약



### 예제



### 연습 문제

> #### [1 ~ 10] Justify each step, using commutativity and associativity in proving the following identities.
>
> #### 1. $$(a + b) + (c + d) = (a + d) + (b + c)$$
>
> \begin{align\*} 
> (a + b) + (c + d) &= a + b + c + d & \text{by associativity} \\\\ 
> &= a + d + b + c & \text{by commutativity} \\\\ 
> &= (a + d) + (b + c) & \text{by associativity}
> \end{align\*}
>
> $$\therefore (a + b) + (c + d) = (a + d) + (b + c)$$
>
> #### 2. $$(a + b) + (c + d) = (a + c) + (b + d)$$
>
> \begin{align\*} 
> (a + b) + (c + d) &= a + b + c + d & \text{by associativity} \\\\ 
> &= a + c + b + d & \text{by commutativity} \\\\ 
> &= (a + c) + (b + d) & \text{by associativity}
> \end{align\*}
>
> #### [14 ~ 21] Solve for $$x$$ in the following equations.
>
> #### 14. $$-2 + x = 4$$
>
> $$-2 + x + 2 = 4 + 2$$
>
> $$x + (-2) + 2 = 4 + 2$$
>
> $$x + \cancel{(-2) + 2} = 4 + 2$$
>
> $$\therefore x = 6$$
>
> #### 15. $$2 - x = 5$$
>
> $$2 - x + x = 5 + x$$
>
> $$2 +\cancel{(-x) + x} = 5 + x$$
>
> $$2 = 5 + x$$
>
> $$2 - 5 = 5 - 5 + x$$
>
> $$-3 = \cancel{5 - 5} + x$$
>
> $$\therefore x = -3$$